qcp/ast/VC/subst_proof_manual.v
@@ -15,9 +15,8 @@ Local Open Scope Z_scope.
 Local Open Scope sets.
 Local Open Scope string.
 Local Open Scope list.
-Require Import ast_lib.
-Require Import Coq.Strings.String.
-Require Import ast_lib.
+Import naive_C_Rules.
+From SimpleC.EE Require Import ast_lib.
 From SimpleC.EE Require Import malloc.
 From SimpleC.EE Require Import sll_tmpl.
 Local Open Scope sac.
@@ -26,89 +25,282 @@ Lemma proof_of_subst_var_return_wit_1_1 : subst_var_return_wit_1_1.
 Proof. Admitted. 
 
 Lemma proof_of_subst_var_return_wit_1_2 : subst_var_return_wit_1_2.
-Proof. Admitted. 
+Proof.
+    pre_process.
+    unfold list_Z_cmp in H0.
+    rewrite H in H0.
+    destruct (list_Z_eqb qvar src_str) eqn:Heq; [ | discriminate ].
+    unfold term_subst_v.
+    rewrite H1, Heq.
+    unfold store_term at 2.
+    simpl.
+    fold store_term.
+    Exists y z. 
+    entailer!.
+Qed. 
 
 Lemma proof_of_subst_var_return_wit_1_3 : subst_var_return_wit_1_3.
-Proof. Admitted. 
+Proof.
+    pre_process.
+    unfold list_Z_cmp in H1.
+    destruct (list_Z_eqb qvar src_str) eqn:Heq; [ contradiction | ].
+    unfold term_subst_v.
+    rewrite H2, Heq.
+    fold term_subst_v.
+    unfold store_term at 2.
+    simpl.
+    fold store_term.
+    Exists y z.
+    rewrite H.
+    entailer!.
+Qed. 
 
 Lemma proof_of_subst_var_return_wit_1_4 : subst_var_return_wit_1_4.
-Proof. Admitted. 
+Proof.
+    pre_process.
+    unfold term_subst_v at 3.
+    rewrite H1.
+    fold term_subst_v.
+    unfold store_term at 3.
+    simpl.
+    fold store_term.
+    Exists y z.
+    rewrite H, H0.
+    entailer!.
+Qed.
 
 Lemma proof_of_subst_var_return_wit_1_5 : subst_var_return_wit_1_5.
-Proof. Admitted. 
+Proof. 
+    pre_process.
+    unfold term_subst_v.
+    rewrite H.
+    unfold store_term.
+    entailer!.
+Qed.
 
 Lemma proof_of_subst_var_return_wit_1_6 : subst_var_return_wit_1_6.
-Proof. Admitted. 
-
+Proof.
+    pre_process.
+    unfold list_Z_cmp in H0.
+    destruct (list_Z_eqb var src_str) eqn:Heq; [ contradiction | ].
+    unfold term_subst_v.
+    rewrite H1, Heq.
+    unfold store_term.
+    Exists y.
+    entailer!.
+Qed.
+    
 Lemma proof_of_subst_var_return_wit_1_7 : subst_var_return_wit_1_7.
-Proof. Admitted. 
-
+Proof. 
+    pre_process.
+    unfold list_Z_cmp in H1.
+    rewrite H0 in H1.
+    destruct (list_Z_eqb var src_str) eqn:Heq; [ | discriminate ].
+    unfold term_subst_v.
+    rewrite H2, Heq.
+    unfold store_term.
+    Exists retval.
+    entailer!.
+Qed.
+    
 Lemma proof_of_subst_var_partial_solve_wit_4_pure : subst_var_partial_solve_wit_4_pure.
-Proof. Admitted. 
-
-Lemma proof_of_subst_var_partial_solve_wit_7_pure : subst_var_partial_solve_wit_7_pure.
-Proof. Admitted. 
+Proof.
+    pre_process.
+    unfold store_string.
+    entailer!. 
+    
+    Admitted. 
 
 Lemma proof_of_subst_var_partial_solve_wit_8_pure : subst_var_partial_solve_wit_8_pure.
-Proof. Admitted. 
+Proof. 
+    pre_process. Admitted. 
 
-Lemma proof_of_subst_var_partial_solve_wit_11_pure : subst_var_partial_solve_wit_11_pure.
-Proof. Admitted. 
+Lemma proof_of_subst_var_partial_solve_wit_9_pure : subst_var_partial_solve_wit_9_pure.
+Proof.
+    pre_process. Admitted. 
+
+Lemma proof_of_subst_var_partial_solve_wit_12_pure : subst_var_partial_solve_wit_12_pure.
+Proof.
+    pre_process.
+    entailer!. Admitted. 
 
 Lemma proof_of_subst_var_which_implies_wit_1 : subst_var_which_implies_wit_1.
-Proof. Admitted. 
+Proof. 
+    pre_process.
+    sep_apply store_term_unfold.
+    entailer!.
+Qed.
 
 Lemma proof_of_subst_var_which_implies_wit_2 : subst_var_which_implies_wit_2.
-Proof. Admitted. 
+Proof.
+    pre_process.
+    sep_apply store_term'_Var; [ | tauto].
+    Intros var y.
+    Exists y var.
+    entailer!.
+Qed. 
 
 Lemma proof_of_subst_var_which_implies_wit_3 : subst_var_which_implies_wit_3.
-Proof. Admitted. 
+Proof. 
+    pre_process.
+    sep_apply store_term'_Const; [ | tauto].
+    Intros y z.
+    Exists y z.
+    entailer!.
+Qed. 
 
 Lemma proof_of_subst_var_which_implies_wit_4 : subst_var_which_implies_wit_4.
-Proof. Admitted. 
+Proof. 
+    pre_process.
+    sep_apply store_term'_Apply; [ | tauto].
+    Intros lt rt y z.
+    Exists z y lt rt.
+    entailer!.
+Qed.
+
+Lemma proof_of_subst_var_which_implies_wit_5 : subst_var_which_implies_wit_5.
+Proof. 
+    pre_process.
+    sep_apply store_term'_Quant; [ | tauto].
+    Intros typ v b y z.
+    Exists z y typ v b.
+    entailer!.
+Qed. 
 
 Lemma proof_of_subst_term_return_wit_1_1 : subst_term_return_wit_1_1.
-Proof. Admitted. 
+Proof. 
+    pre_process.
+    Admitted.
 
 Lemma proof_of_subst_term_return_wit_1_2 : subst_term_return_wit_1_2.
-Proof. Admitted. 
-
+Proof.
+    pre_process.
+    unfold list_Z_cmp in H0.
+    rewrite H in H0.
+    destruct (list_Z_eqb qvar src_str) eqn:Heq; [ | discriminate ].
+    unfold term_subst_t.
+    rewrite H1, Heq.
+    unfold store_term at 3.
+    fold store_term.
+    Exists y z. 
+    entailer!.
+Qed.
+    
 Lemma proof_of_subst_term_return_wit_1_3 : subst_term_return_wit_1_3.
-Proof. Admitted. 
+Proof. 
+    pre_process.
+    unfold list_Z_cmp in H0.
+    destruct (list_Z_eqb qvar src_str) eqn:Heq; [ contradiction | ].
+    unfold term_subst_t.
+    rewrite H1, Heq.
+    fold term_subst_t.
+    unfold store_term at 3.
+    fold store_term.
+    Exists y retval.
+    entailer!.
+Qed.
 
 Lemma proof_of_subst_term_return_wit_1_4 : subst_term_return_wit_1_4.
-Proof. Admitted. 
+Proof. 
+    pre_process.
+    unfold term_subst_t at 3.
+    rewrite H.
+    fold term_subst_t.
+    unfold store_term at 4.
+    fold store_term.
+    Exists retval_2 retval.
+    entailer!.
+Qed.
 
 Lemma proof_of_subst_term_return_wit_1_5 : subst_term_return_wit_1_5.
-Proof. Admitted. 
+Proof. 
+    pre_process.
+    unfold term_subst_t.
+    rewrite H.
+    unfold store_term at 2.
+    entailer!.
+Qed.
 
 Lemma proof_of_subst_term_return_wit_1_6 : subst_term_return_wit_1_6.
-Proof. Admitted. 
+Proof. 
+    pre_process.
+    unfold list_Z_cmp in H0.
+    destruct (list_Z_eqb var src_str) eqn:Heq; [ contradiction | ].
+    unfold term_subst_t.
+    rewrite H2, Heq.
+    unfold store_term at 2.
+    Exists y.
+    entailer!.
+Qed.
 
 Lemma proof_of_subst_term_return_wit_1_7 : subst_term_return_wit_1_7.
-Proof. Admitted. 
-
-Lemma proof_of_subst_term_partial_solve_wit_8_pure : subst_term_partial_solve_wit_8_pure.
-Proof. Admitted. 
+Proof. 
+    pre_process.
+    unfold list_Z_cmp in H1.
+    rewrite H0 in H1.
+    destruct (list_Z_eqb var src_str) eqn:Heq; [ | discriminate ].
+    unfold term_subst_t.
+    rewrite H3, Heq.
+    entailer!.
+Qed.
 
 Lemma proof_of_subst_term_partial_solve_wit_9_pure : subst_term_partial_solve_wit_9_pure.
 Proof. Admitted. 
 
-Lemma proof_of_subst_term_partial_solve_wit_12_pure : subst_term_partial_solve_wit_12_pure.
+Lemma proof_of_subst_term_partial_solve_wit_10_pure : subst_term_partial_solve_wit_10_pure.
+Proof. Admitted. 
+
+Lemma proof_of_subst_term_partial_solve_wit_13_pure : subst_term_partial_solve_wit_13_pure.
 Proof. Admitted. 
 
 Lemma proof_of_subst_term_which_implies_wit_1 : subst_term_which_implies_wit_1.
-Proof. Admitted. 
+Proof. 
+    pre_process.
+    sep_apply store_term_unfold.
+    entailer!.
+Qed.
 
 Lemma proof_of_subst_term_which_implies_wit_2 : subst_term_which_implies_wit_2.
-Proof. Admitted. 
+Proof. 
+    pre_process.
+    sep_apply store_term'_Var; [ | tauto].
+    Intros var y.
+    Exists y var.
+    entailer!.
+Qed. 
 
 Lemma proof_of_subst_term_which_implies_wit_3 : subst_term_which_implies_wit_3.
-Proof. Admitted. 
+Proof. 
+    pre_process.
+    rewrite H0.
+    unfold store_term.
+    Exists y.
+    entailer!.
+Qed.
 
 Lemma proof_of_subst_term_which_implies_wit_4 : subst_term_which_implies_wit_4.
-Proof. Admitted. 
+Proof.
+    pre_process.
+    sep_apply store_term'_Const; [ | tauto].
+    Intros y z.
+    Exists y z.
+    entailer!.
+Qed. 
 
 Lemma proof_of_subst_term_which_implies_wit_5 : subst_term_which_implies_wit_5.
-Proof. Admitted. 
+Proof. 
+    pre_process.
+    sep_apply store_term'_Apply; [ | tauto].
+    Intros lt rt y z.
+    Exists z y lt rt.
+    entailer!.
+Qed.
 
+Lemma proof_of_subst_term_which_implies_wit_6 : subst_term_which_implies_wit_6.
+Proof. 
+    pre_process.
+    sep_apply store_term'_Quant; [ | tauto].
+    Intros typ v b y z.
+    Exists z y typ v b.
+    entailer!.
+Qed.
